

Approximation EOS $\epsilon(P)$ from $P(\epsilon)$
 In Vergara et al PRD 2019

Invertible form.

$$P := \frac{1}{3} (\epsilon - 4B) - \alpha (\epsilon - B)^{1/2}$$

$$\Rightarrow \epsilon = \frac{3}{2} \left\{ \sqrt{3} \alpha (3\alpha^2 + 4(B+P))^{1/2} + 3\alpha^2 + 2(B+P) \right\} + B.$$

$$\epsilon = 3(P+B) + \Delta \epsilon(\alpha) + B. \quad (1)$$

With

$$\Delta \epsilon(\alpha, P) = \frac{3\sqrt{3}}{2} \alpha (3\alpha^2 + 4(B+P))^{1/2} + \frac{9}{2} \alpha^2 \quad (2)$$

our case invertible because. [Eq. (1), Vergara et al]

$$P = \frac{1}{3} (\epsilon - 4B) - \alpha (\epsilon - B)^{1/2} + \beta \left[1 + K \ln \left\{ \gamma (\epsilon - B)^{1/2} \right\} \right] \quad (3)$$

Therefore, we approximate eq. (3) by substitute eq. (1) into the last term of eq. (3).

(1).

$$P - \beta \left[1 + K \ln \left\{ \gamma \left[3(P+B) + \Delta E \right]^{1/2} \right\} \right]$$

$$= \frac{1}{3} (E - 4B) - \alpha (E - B)^{1/2}$$

If we define.

$$\tilde{P} := P - \beta \left[1 + K \ln \left\{ \gamma \left[3(P+B) + \Delta E \right]^{1/2} \right\} \right]$$

Then we have inverted form as: (4a)

$$E \approx \frac{3}{2} \left[\sqrt{3} \alpha \left[3\alpha^2 + 4(B + \tilde{P}) \right]^{1/2} + 3\alpha^2 + 2(\tilde{P} + B) \right] + B. \quad (4b)$$

Here:

$$\alpha := \frac{m_s^2}{3\pi} \frac{1}{\sqrt{a_4}}$$

$$\gamma := \frac{8\pi}{3m_s^2} \frac{1}{\sqrt{a_4}}$$

$$\beta := \frac{m_s^4}{12\pi^2} \left(1 - \frac{1}{a_4} \right)$$

$$K := \frac{3}{\left(1 - \frac{2}{a_4} \right)}$$

In Vergara et al.

(2)

eq. (4b) + eq (4) in Vergara et al. we can solve TOV eq. (7) & (8)